theories/Soundness.v
@@ -18,16 +18,15 @@ Section soundness.
   Lemma LS_Ax : forall Γ Δ φ, In φ Γ -> In φ Δ -> Γ ⊫ Δ.
   Proof.
     intros Γ Δ φ Hin1 Hin2 M Hstandard ρ Hsat.
-    exists φ; intuition.
+    exists φ; split; auto.
   Qed.
 
   Lemma LS_Wk : forall Γ' Δ' Γ Δ, Γ' ⊆ Γ -> Δ' ⊆ Δ ->
                              Γ' ⊫ Δ' -> Γ ⊫ Δ.
   Proof.
     intros Γ' Δ' Γ Δ HsubsΓ HsubsΔ Hsat M Hstandard ρ HsatΓ.
-    assert (HsatΓ' : forall φ, In φ Γ' -> Sat ρ φ) by intuition.
-    apply Hsat in HsatΓ' as [ψ [HinΔ' Hsatψ]].
-    exists ψ; auto. auto.
+    assert (HsatΓ' : forall φ, In φ Γ' -> Sat ρ φ) by auto.
+    apply Hsat in HsatΓ' as [ψ [HinΔ' Hsatψ]]; [ exists ψ | ]; auto.
   Qed.
 
   Lemma LS_Cut : forall Γ Δ φ, Γ ⊫ (φ :: Δ) -> (φ :: Γ) ⊫ Δ -> Γ ⊫ Δ.
@@ -35,8 +34,8 @@ Section soundness.
     intros Γ Δ φ Hsat1 Hsat2 M Hstandard ρ HsatΓ.
     pose proof (Hsat1 M Hstandard ρ HsatΓ) as [ψ [Hin Hsatψ]].
     inversion Hin; subst; clear Hin.
-    - apply Hsat2; auto. intros φ Hin'. inversion Hin'; subst; intuition.
-    - exists ψ; intuition.
+    - apply Hsat2; auto. intros φ Hin'. inversion Hin'; subst; auto.
+    - exists ψ; auto.
   Qed.
 
   Lemma LS_Subst : forall Γ Δ, Γ ⊫ Δ -> forall σ, map (subst_formula σ) Γ ⊫ (map (subst_formula σ) Δ).
@@ -55,87 +54,89 @@ Section soundness.
       Γ ⊫ (φ :: Δ) -> (FNeg φ :: Γ) ⊫ Δ.
   Proof.
     intros Γ Δ φ Hsat M Hstandard ρ HsatΓ.
-    assert (HΓ : forall φ, In φ Γ -> ρ ⊨ φ) by intuition.
+    assert (HΓ : forall φ, In φ Γ -> ρ ⊨ φ) by (intros ε Hin; apply HsatΓ; now right).
     apply Hsat in HΓ as [ψ [Hinψ Hsatψ]].
     inversion Hinψ; subst; clear Hinψ.
-    - assert (Hsatnψ : ρ ⊨ (FNeg ψ)) by intuition. contradiction.
+    - assert (Hsatnψ : ρ ⊨ (FNeg ψ)) by (apply HsatΓ; now left); contradiction.
     - exists ψ; auto.
     - auto.
   Qed.
 
-  Lemma LS_NegR : forall Γ Δ φ,      (* NOTE: uses excluded middle *)
+  Lemma LS_NegR : forall Γ Δ φ,
       (φ :: Γ) ⊫ Δ -> Γ ⊫ (FNeg φ :: Δ).
   Proof.
     intros Γ Δ φ Hsatseq M Hstandard ρ HsatΓ.
     pose proof (classic (ρ ⊨ φ)) as [Hsatφ | Hnsatφ].
     - assert (forall ψ, In ψ (φ :: Γ) -> ρ ⊨ ψ).
-      { intros ψ Hin; inversion Hin; subst; intuition. }
+      { intros ψ Hin; inversion Hin; subst; auto. }
       apply Hsatseq in H as [ψ [Hinψ Hsatψ]]; auto.
-      exists ψ; intuition.
-    - exists (FNeg φ); intuition.
+      exists ψ; split; auto. now right.
+    - exists (FNeg φ); split; auto. now left.
   Qed.
 
   Lemma LS_ImpL : forall Γ Δ φ ψ,
       Γ ⊫ (φ :: Δ) -> (ψ :: Γ) ⊫ Δ -> (FImp φ ψ :: Γ) ⊫ Δ.
   Proof.
     intros Γ Δ φ ψ Hsatseq1 Hsatseq2 M Hstandard ρ HsatΓ.
-    assert (Himpsat : ρ ⊨ (FImp φ ψ)) by intuition.
+    assert (Himpsat : ρ ⊨ (FImp φ ψ)) by (apply HsatΓ; now left).
     cbn in Himpsat.
-    assert (HΓ : forall ξ, In ξ Γ -> ρ ⊨ ξ) by intuition;
-      apply Hsatseq1 in HΓ as [ξ [Hinξ Hsatξ]].
+    assert (HΓ : forall ξ, In ξ Γ -> ρ ⊨ ξ) by (intros ξ Hin; apply HsatΓ; now right).
+    apply Hsatseq1 in HΓ as [ξ [Hinξ Hsatξ]]; auto.
     inversion Hinξ; subst; clear Hinξ; auto.
     - apply Himpsat in Hsatξ.
-      assert (H : forall γ, In γ (ψ :: Γ) -> ρ ⊨ γ) by
-        (intros γ Hin; inversion Hin; subst; intuition);
+      assert (H : forall γ, In γ (ψ :: Γ) -> ρ ⊨ γ).
+      { intros γ Hin; destruct Hin; subst; auto. apply HsatΓ; now right. }
         apply Hsatseq2 in H; auto.
     - exists ξ; auto.
-    - auto.
   Qed.
 
-  Lemma LS_ImpR : forall Γ Δ φ ψ,    (* NOTE: uses excluded middle *)
+  Lemma LS_ImpR : forall Γ Δ φ ψ,
       (φ :: Γ) ⊫ (ψ :: Δ) -> Γ ⊫ (FImp φ ψ :: Δ).
   Proof.
     intros Γ Δ φ ψ Hsatseq M Hstandard ρ HsatΓ.
     pose proof (classic (ρ ⊨ φ)) as [Hsatφ | Hnsatφ].
-    - assert (H: forall ξ, In ξ (φ :: Γ) -> ρ ⊨ ξ) by (intros ξ Hinξ; inversion Hinξ; subst; intuition);
+    - assert (H: forall ξ, In ξ (φ :: Γ) -> ρ ⊨ ξ) by (intros ξ Hinξ; inversion Hinξ; subst; auto);
         apply Hsatseq in H as [ξ [Hinξ Hsatξ]].
       inversion Hinξ; subst; clear Hinξ.
-      + exists (FImp φ ξ); cbn; intuition.
-      + exists ξ; intuition.
+      + exists (FImp φ ξ); cbn; auto.
+      + exists ξ; split; auto. now right.
       + auto.
-    - exists (FImp φ ψ); cbn; intuition.
+    - exists (FImp φ ψ); cbn; split; auto; intros contra; contradiction.
   Qed.
     
-  Lemma LS_AllL : forall Γ Δ φ t,    (* NOTE: uses excluded middle *)
+  Lemma LS_AllL : forall Γ Δ φ t,
       (subst_formula (t .: ids) φ :: Γ) ⊫ Δ ->
       (FAll φ :: Γ) ⊫ Δ.
   Proof.
     intros Γ Δ φ t Hsatprem M Hstandard ρ HsatΓ.
-    assert (Hφ : ρ ⊨ (FAll φ)) by intuition. cbn in Hφ.
+    assert (Hφ : ρ ⊨ (FAll φ)) by (apply HsatΓ; now left).
     pose proof (classic (ρ ⊨ (subst_formula (t .: ids) φ))) as [H | H].
-    - assert (HΓ : forall ψ, In ψ (subst_formula (t .: ids) φ :: Γ) -> ρ ⊨ ψ) by (intros ψ Hin; inversion Hin; subst; intuition);
-        apply Hsatprem in HΓ as [ψ [Hinψ Hsatψ]]. exists ψ; intuition. auto.
-    - rewrite strong_form_subst_sanity2 in H. specialize Hφ with (eval ρ t).
-      asimpl in *. contradiction.
+    - assert (HΓ : forall ψ, In ψ (subst_formula (t .: ids) φ :: Γ) -> ρ ⊨ ψ).
+      { intros ψ Hin; inversion Hin; subst; auto. apply HsatΓ; now right. }
+      apply Hsatprem in HΓ as [ψ [Hinψ Hsatψ]]; auto. exists ψ; split; auto.
+    - rewrite strong_form_subst_sanity2 in H.
+      asimpl in *; cbn in Hφ; specialize Hφ with (eval ρ t).
+      contradiction.
   Qed.
 
-  Lemma LS_ExL : forall Γ Δ φ,       (* NOTE: uses excluded middle *)
+  Lemma LS_ExL : forall Γ Δ φ,
       (φ :: shift_formulas Γ) ⊫ (shift_formulas Δ) ->
       (FExist φ :: Γ) ⊫ Δ.
   Proof.
     intros Γ Δ φ Hsat M Hstandard ρ Hsat1.
-    assert (Hexφ : ρ ⊨ (FExist φ)) by intuition.
+    assert (Hexφ : ρ ⊨ (FExist φ)) by (apply Hsat1; now left).
     cbn in Hexφ. apply not_all_not_ex in Hexφ.
     destruct Hexφ as [d Hd].
     assert (HΓ : forall ψ, In ψ (shift_formulas Γ) -> (d .: ρ) ⊨ ψ).
     { intros ψ Hin. apply in_map_iff in Hin as [ξ [Heq Hinξ]]; subst.
-      unfold shift_formula. rewrite strong_form_subst_sanity2.
+      unfold shift_formula_by. rewrite strong_form_subst_sanity2.
       apply Hsat1. now right. }
     assert (H : forall ψ, In ψ (φ :: shift_formulas Γ) -> (d .: ρ) ⊨ ψ) by (intros ψ Hin; inversion Hin; subst; intuition).
     apply Hsat in H; auto.
     destruct H as [ψ [Hinψ Hsatψ]].
     apply in_map_iff in Hinψ as [ξ [Heq Hinξ]]; subst. exists ξ; split. assumption.
-    unfold shift_formula in Hsatψ. rewrite strong_form_subst_sanity2 in Hsatψ. assumption.
+    unfold shift_formula_by in Hsatψ.
+    rewrite strong_form_subst_sanity2 in Hsatψ. assumption.
   Qed.
 
   Lemma LS_ExR : forall Γ Δ φ t,
@@ -149,10 +150,10 @@ Section soundness.
       rewrite strong_form_subst_sanity2 in Hsatψ.
       intros H. specialize H with (eval ρ t).
       apply H. rewrite scons_comp in Hsatψ. auto.
-    - exists ψ; intuition.
+    - exists ψ; split; auto. now right.
   Qed.
 
-  Lemma Semantic_NegExistNegAll : forall Γ Δ φ, (* NOTE: uses XM *)
+  Lemma Semantic_NegExistNegAll : forall Γ Δ φ,
       Γ ⊫ (FNeg (FExist (FNeg φ)) :: Δ) ->
       Γ ⊫ (FAll φ :: Δ).
   Proof.
@@ -186,7 +187,7 @@ Section soundness.
     intros Γ Δ pr σ HΦ Hpreds Hindpreds M Hstandard ρ HsatΓ.
     cbn beta in Hpreds, Hindpreds.
     pose proof (classic (exists ψ, In ψ Δ /\ ρ ⊨ ψ)) as [HΔ | HΔ].
-    - destruct HΔ as [ψ [Hinψ Hsatψ]]; exists ψ; intuition.
+    - destruct HΔ as [ψ [Hinψ Hsatψ]]; exists ψ; split; auto. now right.
     - assert (Hpreds' : forall Q us, In (Q; us) (preds pr) -> ρ ⊨ (FPred Q (V.map (subst_term σ) us))).
       { intros Q us Hin. pose proof (Hpreds Q us Hin M Hstandard ρ HsatΓ) as [ξ [Hinξ Hsatξ]].
         inversion Hinξ; subst; clear Hinξ.
@@ -221,7 +222,7 @@ Section soundness.
       let shift_factor := max maxP (max maxΓ maxΔ) in
       let Fj := subst_formula (finite_subst (z_i Pj) u) (G_i Pj) in
       let minor_premises :=
-        (forall pr (HΦ : Φ pr) (Hdep : @mutually_dependent Σ Φ (indcons pr) Pj),
+        (forall pr (HΦ : Φ pr) (Hdep : mutually_dependent Φ (indcons pr) Pj),
             let Qs := shift_formulas_by shift_factor (FPreds_from_preds (preds pr)) in
             let Gs := map (fun '(P; args) =>
                              let shifted_args := V.map (shift_term_by shift_factor) args in
@@ -241,14 +242,72 @@ Section soundness.
     intros Γ Δ Pj u z_i z_i_nodup G_i HmutdepG.
     intros maxΓ maxΔ maxP shift_factor Fj minor_premises.
     intros Hminor Hindhyp M Hstandard ρ Hpremises.
-    assert (Hsat1 : forall ψ, In ψ Γ -> ρ ⊨ ψ) by intuition.
-    assert (Hsat2: ρ ⊨ (FIndPred Pj u)) by intuition.
-    apply Hstandard in Hsat2.
-    destruct (classic (exists ψ, In ψ Δ /\ ρ ⊨ ψ)) as [H | H].
-    - apply H.
-    - assert (forall ψ, In ψ Δ -> ~ ρ ⊨ ψ) as HΔunsat by (intros ψ HψInΔ Hsatψ; apply H; exists ψ; auto); clear H.
-      
+    assert (Hsat1 : forall ψ, In ψ Γ -> ρ ⊨ ψ).
+    { intros ψ Hin; apply Hpremises; now right. }
+    assert (Hsat2: ρ ⊨ (FIndPred Pj u)).
+    { apply Hpremises; now left. }
+    apply Hindhyp; auto.
+    intros φ [HφFj | HinΓ]; auto; clear Hsat1 Hpremises Hindhyp; subst φ.
+    apply Hstandard in Hsat2 as [[|α] Hsatα]; try contradiction.
+    destruct Hsatα as (pr & [Heq HΦ] & ρ' & Hpreds & Hindpreds & Heval); subst Pj;
+      cbn in Heval.
+    assert (forall t v,
+               eval ρ (subst_term (finite_subst v u) t) =
+                 eval ρ' (subst_term (finite_subst v (indargs pr)) t)).
+    { admit. }
   Admitted.
+  (*   destruct (classic (exists ψ, In ψ Δ /\ ρ ⊨ ψ)) as [H | H]. *)
+  (*   { apply H. } *)
+  (*   assert (forall ψ, In ψ Δ -> ~ ρ ⊨ ψ) as HΔunsat. *)
+  (*   { intros ψ Hin Hsat. apply H; exists ψ; auto. } *)
+  (*   clear H.  *)
+
+  (*   specialize (Hminor pr HΦ (mutually_dependent_refl Φ (indcons pr))). *)
+  (*   cbn in Heval. *)
+  (*   remember (shift_formulas_by shift_factor (FPreds_from_preds (preds pr))) as Qs. *)
+  (*   remember (list_map *)
+  (*              (λ '(P; args), *)
+  (*                 let shifted_args := V.map (shift_term_by shift_factor) args in *)
+  (*                 let σ := finite_subst (z_i P) shifted_args in let G := G_i P in subst_formula σ G) *)
+  (*              (indpreds pr)) as Gs. *)
+  (*   remember (V.map (shift_term_by shift_factor) (indargs pr)) as ty. *)
+  (*   set (Pi := indcons pr). *)
+  (*   assert (HeqPi : Pi = indcons pr) by auto. *)
+  (*   remember (subst_formula (finite_subst (z_i Pi) ty) (G_i Pi)) as Fi. *)
+  (*   cbn in Hminor. *)
+  (*   specialize (Hminor M Hstandard ρ). *)
+  (*   subst Pi; clear HeqPi. *)
+  (*   rewrite <- HeqFi in Hminor. *)
+  (*   enough (H : forall ε, In ε (Qs ++ Gs ++ Γ) -> ρ ⊨ ε). *)
+  (*   { *)
+  (*     apply Hminor in H as [ξ [[H | H] Hξsat]]. *)
+  (*     - apply Hindhyp; auto. intros ψ Hinψ; destruct Hinψ as [HψFj | HinψΓ]. *)
+  (*       + subst ξ. subst ψ. subst Fi. apply strong_form_subst_sanity2 in Hξsat. *)
+  (*         subst Fj. apply strong_form_subst_sanity2. admit. *)
+  (*       + auto. *)
+  (*     - exists ξ; auto. *)
+  (*   } *)
+  (*   intros ψ Hin. *)
+  (*   apply in_app_or in Hin as [HinQs | Hin]. *)
+  (*   { *)
+  (*     subst Qs. *)
+  (*     apply in_map_iff in HinQs as [ξ [Heq Hin]]. *)
+  (*     apply in_map_iff in Hin as [[Q args] [Heq1 Hin]]. *)
+  (*     specialize (Hpreds Q args Hin). subst ψ. *)
+  (*     subst ξ. apply strong_form_subst_sanity2. *)
+  (*     admit. *)
+  (*   } *)
+  (*   apply in_app_or in Hin as [HinGs | HinΓ]. *)
+  (*   - subst Gs. apply in_map_iff in HinGs. *)
+  (*     destruct HinGs as ([P args] & Heq & Hin). *)
+  (*     remember (V.map (shift_term_by shift_factor) args) as shifted_args. *)
+  (*     remember (finite_subst (z_i P) shifted_args) as σ. *)
+  (*     remember (G_i P) as G. cbn in Heq. rewrite <- Heqσ in Heq. *)
+  (*     rewrite <- Heq. apply strong_form_subst_sanity2. *)
+  (*     specialize (Hindpreds P args Hin). *)
+  (*     admit. *)
+  (*   - auto. *)
+  (* Admitted. *)
     
     
   Theorem soundness : forall Γ Δ, @LKID Σ Φ (Γ ⊢ Δ) -> Γ ⊫ Δ.
@@ -258,7 +317,7 @@ Section soundness.
     - apply LS_Ax with Γ0 φ; auto.
     - apply LS_Wk with Γ' Δ' Γ0; auto.
     - apply LS_Cut with Γ0 φ; auto.
-    - eapply LS_Subst; eauto.
+    - now apply (LS_Subst Γ0 Δ0 IHHlkid σ M Hstandard ρ).
     - eapply LS_NegL; eauto.
     - eapply LS_NegR; eauto.
     - eapply LS_ImpL; eauto.
